lean/gc/Gc/Model/Start.lean
@@ -116,6 +116,13 @@ theorem RuntimeConfig.start_HS1 : HS1 RuntimeConfig.start := by
   dsimp at hmem
   simp at hmem
 
+theorem RuntimeConfig.start_HS2 : HS2 RuntimeConfig.start := by
+  unfold HS2
+  intro rid hmem
+  unfold RuntimeConfig.start RuntimeConfig.refs Stack.refs Frame.refs Heap.refs Region.refs Object.refs at hmem
+  dsimp at hmem
+  simp at hmem
+
 theorem RuntimeConfig.start_valid : ValidConfig RuntimeConfig.start :=
   { l1 := RuntimeConfig.start_L1,
     l2 := RuntimeConfig.start_L2,
@@ -126,4 +133,5 @@ theorem RuntimeConfig.start_valid : ValidConfig RuntimeConfig.start :=
     s2 := RuntimeConfig.start_valid_S3,
     s3 := RuntimeConfig.start_valid_S4,
     hs1 := RuntimeConfig.start_HS1,
+    hs2 := RuntimeConfig.start_HS2,
   }
